$$
\def\mysum#1{\sum\limits#1}
\def\l#1{\left#1}
\def\r#1{\right#1}
\def\({\l(}
\def\){\r)}
\def\[{\l\lbrack}
\def\]{\r\rbrack}
\def\{{\l\lbrace}
\def\}{\r\rbrace}
$$

对于命题 $P$，记 $
\[P\]=
\begin{cases}
1,&P\text{ 为真}
\\
0,&P\text{ 为假}
\end{cases}
$。

对于关于 $x$ 的多项式 $f(x)$，记 $\[x^i\]f(x)$ 为 $f(x)$ 的 $i$ 次项系数。

---

求证：$f(n) = \mysum_{i=0}^{n}\binom{n}{i}g(i) \Leftrightarrow g(n) = \mysum_{i=0}^{n}{(-1)^{n-i}\binom{n}{i}f(i)}$。

---

两点引理：

$
\begin{aligned}
&\mysum_{i=0}^{n}{(-1)^{i}\binom{n}{i}}
\\
=& \mysum_{i=0}^{n}{\[x^i\](1-x)^n}
\\
=& \(1-x\)^n\big|_{x=1}
\\
=& \[n=0\]
\end{aligned}
$

$
\begin{aligned}
&\binom{n}{m}\binom{n-m}{k}
\\
=&\frac{n!}{m!(n-m)!} \times \frac{(n-m)!}{k!((n-m)-k)!}
\\
=&\frac{n!}{k!(n-k)!} \times \frac{(n-k)!}{m!((n-k)-m)!}
\\
=&\binom{n}{k}\binom{n-k}{m}
\end{aligned}
$

---

先证 $f(n) = \mysum_{i=0}^{n}\binom{n}{i}g(i) \Rightarrow g(n) = \mysum_{i=0}^{n}{(-1)^{n-i}\binom{n}{i}f(i)}$。

$$
\begin{aligned}
g(n)
&= \mysum_{m=0}^{n-1}0+\mysum_{m=n}^{n}{\binom{n}{m}g(m)}
\\
&= \mysum_{m=0}^{n}{\[n-m=0\]\binom{n}{m}g(m)}
\\
&= \mysum_{m=0}^{n}{\(\mysum_{i=0}^{n-m}{(-1)^{i}\binom{n-m}{i}}\)\(\binom{n}{m}g(m)\)}
\\
&= \mysum_{m=0}^{n}\mysum_{i=0}^{n-m}{(-1)^{i}\binom{n}{m}\binom{n-m}{i}g(m)}
\\
&= \mysum_{m=0}^{n}{\mysum_{i=0}^{n-m}{(-1)^{i}\binom{n}{i}\binom{n-i}{m}g(m)}}
\\
&\sout{\text{（由打表得）}}
\\
&= \mysum_{i=0}^{n}{\mysum_{m=0}^{n-i}{(-1)^{i}\binom{n}{i}\binom{n-i}{m}g(m)}}
\\
&= \mysum_{i=0}^{n}{\((-1)^{i}\binom{n}{i}\)\(\mysum_{m=0}^{n-i}\binom{n-i}{m}g(m)\)}
\\
&= \mysum_{i=0}^{n}{(-1)^{i}\binom{n}{i}f(n-i)}
\\
&= \mysum_{i=0}^{n}{(-1)^{n-i}\binom{n}{i}f(i)}
\end{aligned}
$$

综上，$f(n) = \mysum_{i=0}^{n}\binom{n}{i}g(i) \Rightarrow g(n) = \mysum_{i=0}^{n}{(-1)^{n-i}\binom{n}{i}f(i)}$ 得证。

---

显然，上述推导过程可逆，故原命题得证。